
\begin{equation} 
    \left\{\begin{array}{l}{\dot{u}=\mathrm{f}(u, t)} \\ {u\left(t_{0}\right)=u_{0}}\end{array}\right.
\end{equation}

\begin{equation} 
    \dot{u}=a u \rightarrow \frac{u_{n+1}-u_{n}}{\Delta t}=a u_{n}
\end{equation}

\begin{equation} 
    \frac{u_{n+1}-u_{n}}{\mathrm{d} t}=\mathrm{f}\left(u^{*}\right)
\end{equation}

\begin{equation} 
    \left\{\begin{array}{l}{\dot{y}=y \sin (t)^{2}} \\ {y(0)=0}\end{array}\right. \Rightarrow y(t)=\exp \left(\frac{t}{2}-\frac{\sin (2 t)}{4}\right)
\end{equation}

\begin{equation} 
    \left\{\begin{array}{l}{\dot{y}=y^{2}} \\ {y(0)=0.1}\end{array}\right. \Rightarrow y(t)=\frac{0.1}{1-0.1 t}
\end{equation}

\begin{equation} 
    \begin{array}{c}{\dot{u}(t)=A u(t)} \\ {A=\left(a_{i j}\right) \in \mathbb{C}} \\ {\Re\left(\lambda_{i}\right)<0 \forall i}\end{array}
\end{equation}

\begin{equation} 
    \left\{\begin{array}{ll}{\dot{u}=\mathrm{f}(u, t)} & {\mathrm{f}(u, t)=\mathrm{A} u+\mathrm{g}(u, t)} \\ {u\left(t_{0}\right)=u_{0}}\end{array}\right. \quad \rightarrow \quad \mathrm{f}(u, t)=\mathrm{A} u+\mathrm{g}(u, t)
\end{equation}

\begin{equation} 
    u(t)=e^{\mathrm{A}\left(t-t_{0}\right)} u_{0}+\int_{t_{0}}^{t} e^{\mathrm{A}(t-s)} \mathrm{g}(u(s), s) \mathrm{d} s
\end{equation}

\begin{equation} 
    u\left(t_{n}+\tau\right)=\mathrm{e}^{-\tau A} u\left(t_{n}\right)+\int_{0}^{\tau} \mathrm{e}^{-(\tau-\sigma) A} g\left(u\left(t_{n}+\sigma\right)\right) d \sigma
\end{equation}

\begin{equation} 
    \begin{aligned} u_{n+1} &=\mathrm{e}^{-\tau A} u_{n}+\tau \sum_{i=1}^{s} b_{i}(-\tau A) G_{n i} \\ G_{n i} &=g\left(U_{n i}\right) \\ U_{n i} &=\mathrm{e}^{-c_{t} \tau A} u_{n}+\tau \sum_{j=1}^{s} a_{i j}(-\tau A) G_{n j} \end{aligned}
\end{equation}

\begin{equation} 
    u\left(t_{n}+\theta \tau\right)=\mathrm{e}^{-\theta \tau A} u\left(t_{n}\right)+\theta \tau \varphi_{1}(-\theta \tau A) g
\end{equation}

\begin{equation} 
    \varphi_{1}(z)=\int_{0}^{1} \mathrm{e}^{(1-\sigma) z} d \sigma=\frac{\mathrm{e}^{z}-1}{z}
\end{equation}

\begin{equation} 
    \begin{array}{l}{\sum_{i=1}^{s} b_{i}(z)=\varphi_{1}(z)} \\ {\sum_{j=1}^{s} a_{i j}(z)=c_{i} \varphi_{1}\left(c_{i} z\right), \quad i=1, \ldots, s}\end{array}
\end{equation}

\begin{equation} 
    g(\tau, u(\tau)) \approx \sum_{k=0}^{p-1} \frac{\left(\tau-t_{0}\right)^{k}}{k !} \frac{\mathrm{d}^{k}}{\mathrm{d} t^{k}} g\left.(t, u(t))\right|_{t=t_{0}}
\end{equation}

\begin{equation} 
    w_{k} \approx \frac{\mathrm{d}^{k-1}}{\mathrm{d} t^{k-1}} g\left.(t, u(t))\right|_{t=t_{0}}
\end{equation}

\begin{equation} 
    u_{1}=\mathrm{e}^{I A} u_{0}+\sum_{k=1}^{p} h^{k} \varphi_{k}(h A) w_{k} = u_{0}+h \varphi_{1}(h A) f\left(t_{0}, u_{0}\right)+\sum_{k=2}^{p} h^{k} \varphi_{k}(h A) w_{k}
\end{equation}

\begin{equation} 
    \varphi_{k}(z)=\int_{0}^{1} \mathrm{e}^{(1-\theta) z} \frac{\theta^{k-1}}{(k-1) !} \mathrm{d} \theta \quad k \geq 1
\end{equation}

\begin{equation} 
    \begin{aligned} u_{n+1} &=\mathrm{e}^{-\tau A} u_{n}+\tau \varphi_{1}(-\tau A) g\left(t_{n}, u_{n}\right) \\ &=\left(I-\tau A \varphi_{1}(-\tau A)\right) u_{n}+\tau \varphi_{1}(-\tau A) g\left(t_{n}, u_{n}\right) \\ &=u_{n}+\tau \varphi_{1}(-\tau A) F\left(t_{n}, u_{n}\right) \end{aligned}
\end{equation}

\begin{equation} 
    F(u(t))=-A u(t)+g(u(t)), \quad A \approx-\frac{\partial F}{\partial u}\left(u_{0}\right)
\end{equation}

\begin{equation} 
    \begin{aligned} F(u(t)) &=-A_{n} u(t)+g_{n}(u(t)) \\ A_{n} &=-\frac{\partial F}{\partial u}\left(u_{n}\right) \end{aligned} \quad n=0,1, \ldots
\end{equation}